no_sig api in progress

share/pulse/examples/dice/dpe/SPDM3.fst
@@ -14,6 +14,7 @@ module V = Pulse.Lib.Vec
 module FP = Pulse.Lib.PCM.FractionalPreorder
 module L = FStar.List.Tot
 module E = FStar.Endianness
+module O = Pulse.Lib.OnRange
 
 open FStar.Mul
 open Pulse.Lib.Pervasives
@@ -44,15 +45,6 @@ open Pulse.Lib.OnRange
 
 let trace_ref = admit ()
 
-let init _ _ = admit ()
-
-let init_inv (key_len:u32) (b:Seq.seq u8) (s:state) (r:gref) : slprop =
-  exists* (t:trace).
-    spdm_inv s r t ** 
-    pure (G_Initialized? (current_state t) /\
-          g_key_of_gst (current_state t) == b /\
-          g_key_len_of_gst (current_state t) == key_len)
-
 let pcm_elt (p:perm) (t:trace) : pcm_t = Some p, t
 
 fn init0 (key_size:u32) (signing_pub_key:V.vec u8 { V.length signing_pub_key == U32.v key_size })
@@ -61,127 +53,275 @@ fn init0 (key_size:u32) (signing_pub_key:V.vec u8 { V.length signing_pub_key == 
   returns r:state & gref
   ensures init_inv key_size s (fst r) (snd r)
 {
+  //creation of session_transcript
   let session_transcript = V.alloc 0uy 0sz;
   
+  //creation of the session data storage
   let st = { key_size; signing_pub_key; session_transcript };
   
+  //creation of the ghost session data storage
   let repr = {key_size_repr = key_size; signing_pub_key_repr = s; transcript = Seq.empty};
   
+  //creation of the trace
   let trace = next_trace emp_trace (G_Initialized repr);
   
+  //creation of the ghost trace ref
   let r = ghost_alloc #_ #trace_pcm (pcm_elt 1.0R trace);
-
+ 
+  (*Current context:
+    ghost_pcm_pts_to r (G.reveal (G.hide (pcm_elt 1.0R trace))) **
+    V.pts_to session_transcript (Seq.Base.create (SZ.v 0sz) 0uy) **
+    V.pts_to signing_pub_key s*)
+  
+  (*We get, V.pts_to signing_pub_key s from the pre-condition. To prove session_related, we need to rewrite signing_pub_key as 
+    st.signing_pub_key and s as repr.signing_pub_key_repr, where rewrite works as these entities are equal*)
   rewrite each
     signing_pub_key as st.signing_pub_key,
     s as repr.signing_pub_key_repr;
 
+   (*Current context:
+    ghost_pcm_pts_to r (G.reveal (G.hide (pcm_elt 1.0R trace))) **
+    V.pts_to session_transcript (Seq.Base.create (SZ.v 0sz) 0uy) **
+    V.pts_to st.signing_pub_key repr.signing_pub_key_repr*)
+
+  (*pure things are asserted with assert_*)
   assert_ (pure (Seq.equal (Seq.create (SZ.v 0sz) 0uy) Seq.empty));
+
+  (*Here, rewrite is for entire V.pts_to, hence use with _v., where _v indicates the seq equivalent of the vector*)
   with _v. rewrite (V.pts_to session_transcript _v) as
                    (V.pts_to st.session_transcript Seq.empty);
+
+   (*Current context:
+    ghost_pcm_pts_to r (pcm_elt 1.0R trace) **
+    V.pts_to st.session_transcript Seq.Base.empty **
+    V.pts_to st.signing_pub_key repr.signing_pub_key_repr*)
+  
+  (*fold with exact values. Otherwise a match block might need to be invoked.*)
   fold (session_state_related (Initialized st) (G_Initialized repr));
+
+  (*Current context:
+    ghost_pcm_pts_to r (pcm_elt 1.0R trace) **
+    session_state_related (Initialized st) (G_Initialized repr)*)
+  
+  (*Since all the conditions for spdm_inv are in the context now, fold spdm_inv*)
   fold (spdm_inv (Initialized st) r trace);
+
+   (*Current context:
+    spdm_inv (Initialized st) r trace*)
+
   let res = (Initialized st, r);
+
+  (*Current context:
+    pure (res == (Initialized st, r)) ** spdm_inv (Initialized st) r trace*)
+
   fold (init_inv key_size s (fst res) (snd res));
+
+  (*Current context:
+    init_inv key_size s (fst res) (snd res)*)
+
   res
 }
 
-(*rewrite each
-        ctr as (fst ret).st_ctr,
-        tbl as (fst ret).st_tbl;*)
+let b_resp_resp_repr_relation (req_param1: u8)
+                              (req_param2:u8) (measurementspecification: u8) 
+                              (req_context: Seq.seq u8{Seq.length req_context == 8})
+                              (r:resp_repr req_param1 req_param2 measurementspecification req_context) (s:Seq.seq u8) =
 
+admit()
 
-(*fold (dpe_inv r None);*)
+let valid_resp_bytes (req_param1: u8)
+                            (req_param2:u8) (measurementspecification: u8) 
+                            (req_context: Seq.seq u8{Seq.length req_context == 8})
+                            (b:Seq.seq u8) 
+                            (r:resp_repr req_param1 req_param2 measurementspecification req_context) =
+admit()
 
-(*let spdm_inv (s:state) (r:gref) (t:trace) : slprop =
-  ghost_pcm_pts_to r (Some 1.0R, t) **
-  session_state_related s (current_state t)*)
-
-(*let session_state_related (s:state) (gs:g_state) : slprop =
-  match s, gs with
-  | Initialized st, G_Initialized repr ->
-    V.pts_to st.signing_pub_key repr.signing_pub_key_repr **
-    V.pts_to st.session_transcript Seq.empty **
-    pure (st.key_size == repr.key_size_repr)
-
-  | Recv_no_sign_resp st, G_Recv_no_sign_resp repr ->
-    V.pts_to st.signing_pub_key repr.signing_pub_key_repr **
-    V.pts_to st.session_transcript repr.transcript **
-    pure (st.key_size == repr.key_size_repr)
-
-  | _ -> pure False
-
-//*)
-
-
-// We assume a combinator to run pulse computations for initialization of top-level state, it gets primitive support in extraction
-assume val run_stt (#a:Type) (#post:a -> slprop) (f:stt a emp post) : a
-
-// We assume this code will be executed on a machine where u32 fits the word size
-assume SZ_fits_u32 : SZ.fits_u32
-
-
-
-fn __init (s:state) (t:trace) (key_len:u32) (signing_key:V.vec u8 { V.length signing_key == U32.v key_len})
-  requires spdm_inv s trace_ref t
-  returns r:(st & state)
-  ensures spdm_inv (snd r) trace_ref t **
-          (exists* p b. V.pts_to signing_key #p b **
-                   init_client_perm (snd r) b key_len)
-
-
-
-assume val emptyVector : v:V.vec u8{V.length v = 0}
- 
- //since the pre-condition has V.pts_to signing_key #p b. post-condition also has that
- //how to bring in init_client_perm r b key_len?
- //how to bring in b? That is the seq version of signing_key
-
-fn init1  (key_len:u32) (signing_key:V.vec u8 { V.length signing_key == U32.v key_len })
-  requires (exists* p b. V.pts_to signing_key #p b)
-  returns r:(state)
-  ensures (exists* p b. V.pts_to signing_key #p b ** 
-                                        init_client_perm r b key_len)
+fn parser 
+  (req_param1: u8)
+  (req_param2 : u8)
+  (resp_size: u8)
+  (m_spec: u8) 
+  (req_context: Seq.seq u8{Seq.length req_context == 8})
+  (resp:V.vec u8 { V.length resp == u8_v resp_size })
+  (signature_size: u8)
+  
+    requires exists* p_resp b_resp. V.pts_to resp #p_resp b_resp
+    returns res: spdm_measurement_result_t 
+    ensures 
+     exists* p_resp b_resp. V.pts_to resp #p_resp b_resp **
+                           (match res.status with
+                            | Parse_error -> pure True
+                            | Signature_verification_error -> pure False
+                            | Success ->
+                              exists* resp_repr. valid_resp_bytes req_param1 req_param2 m_spec req_context b_resp resp_repr **
+                              valid_measurement_blocks req_param2 m_spec res.measurement_block_vector resp_repr.measurement_record)
 {
-   let st =  { key_size = key_len; signing_pub_key = signing_key; session_transcript = emptyVector};
-   Initialized st;
-   _assume (valid_transition emp_trace G_UnInitialized);
-   ghost_write trace_ref (None, emp_trace);
-   ghost_write trace_ref (None, emp_trace) 
-                         (Some 1.0R, (next_trace emp_trace G_UnInitialized));
-   ghost_write trace_ref (Some 1.0R, (next_trace emp_trace G_UnInitialized))
-                         (Some 1.0R, (next_trace emp_trace G_Initialized));
-   admit()
-} 
+  admit()
+}
+
+(*noeq
+type state =
+  | Initialized : st -> state
+  | Recv_no_sign_resp : st -> state*)
+
+(*noeq
+type st = {
+  key_size : u32;
+  signing_pub_key : v:V.vec u8 { V.length v == U32.v key_size };
+  session_transcript : V.vec u8;
+}*)
 
 
-(*noextract
-let next_trace (t:trace) (s:g_state { valid_transition t s }) : trace =
-  match t with
-  | [] -> [[s]]
-  | hd::tl ->
-    match hd with
-    | [] -> [s]::t
-    | l -> (s::l)::t //t == l::tl
+fn get_state_data (c:state)
+requires emp
+returns s:st
+ensures emp
+{
+  match c {
+    Initialized s-> {
+      s
+    }
+    Recv_no_sign_resp s -> {
+      s
+    } 
+  }
+}
+
+fn get_state_data_transcript (s_data:st)
+requires emp
+returns v:V.vec u8
+ensures emp
+{
+  s_data.session_transcript
+}
+
+fn get_state_data_signing_pub_key (s_data:st)
+requires emp
+returns v:V.vec u8
+ensures emp
+{
+  s_data.signing_pub_key
+}
+
+fn get_state_data_key_size (s_data:st)
+requires emp
+returns k:u32
+ensures emp
+{
+  s_data.key_size
+}
+
+//We have taken permissions on v1 and v2 and if we are not returning v1 nad v2, then the client losts this permission and then
+//the client will not be able to deallocate v1 and v2. Read permissions.
+fn append_vec
+  (#a:Type0)
+  (v1: V.vec a)
+  (v2: V.vec a)
+  (#v1_seq: Ghost.erased (Seq.seq a)) //put G.erased
+  (#v2_seq: Ghost.erased (Seq.seq a))
+  (#p1:perm)
+  (#p2:perm)
+  
+  requires V.pts_to v1 #p1 v1_seq **
+           V.pts_to v2 #p2 v2_seq
+
+  returns v:V.vec a
+  ensures V.pts_to v (Seq.append v1_seq v2_seq) **
+          V.pts_to v1 #p1 v1_seq **
+          V.pts_to v2 #p2 v2_seq
+  {
+    admit()
+  }      
+
+(*ghost
+fn current_state_transcript_points_to_trace_current_transcript
+  (c:state)
+  (#tr0:trace{has_full_state_info (current_state tr0)})
+  
+  requires  spdm_inv c trace_ref tr0 
+  ensures   spdm_inv c trace_ref tr0  ** V.pts_to (get_state_data_transcript (get_state_data c)) (current_transcript tr0)
+{
+  admit()
+}
 *)
 
+fn no_sign_resp1
+  (req_param1: u8)
+  (req_param2 : u8)
+  (m_spec: u8) 
+  (req_context: Seq.seq u8{Seq.length req_context == 8})
+  (req_size: u32)
+  (resp_size: u32)
+  (req:V.vec u8 { V.length req == u32_v req_size })
+  (resp:V.vec u8 { V.length resp == u32_v resp_size })
+  (c:state)
+  (#tr0:trace{has_full_state_info (current_state tr0)})
+  (#b_resp: Seq.seq u8)
+  (#b_req: Seq.seq u8)
+  (#p_req : perm)
+  (#p_resp:perm)
+   requires (V.pts_to req #p_req b_req **
+             V.pts_to resp #p_resp b_resp) **
+             spdm_inv c trace_ref tr0 **
+             pure (G_Recv_no_sign_resp? (current_state tr0) \/ G_Initialized? (current_state tr0))
+    returns res: spdm_measurement_result_t 
+    
+    ensures V.pts_to req #p_req b_req **
+            V.pts_to resp #p_resp b_resp **
+            (let measurement_block_count = res.measurement_block_count in
+            let result = res.status in
+                  (match result with
+                    | Parse_error -> pure True
+                    | Signature_verification_error -> pure False
+                    | Success ->
+                              //parser post-condition 
+                              (exists* resp_repr. valid_resp_bytes req_param1 req_param2 m_spec req_context b_resp resp_repr **
+                                       valid_measurement_blocks req_param2 m_spec res.measurement_block_vector resp_repr.measurement_record) **
+                              
+                              //state change related post-condition 
+                              (exists* r tr1. valid_resp req_param1 req_param2 m_spec req_context resp r **
+                                        spdm_inv c trace_ref tr1 **
+                                        (pure (G_Recv_no_sign_resp? (current_state tr1) /\
+                                              valid_transition tr0 (current_state tr1) /\ tr1 == next_trace tr0 (current_state tr1))) **
+                                        (pure (G_Recv_no_sign_resp? (current_state tr1) /\
+                                               
+                                               g_transcript_current_session_grows_by (current_transcript tr0 ) 
+                                                                                     (current_transcript tr1) 
+                                                                                     (Seq.append b_req b_resp))))))
+{
+  //current state transcript
+  let curr_state_data = get_state_data c;
+  let curr_state_transcript = get_state_data_transcript curr_state_data;
+  let curr_state_signing_pub_key = get_state_data_signing_pub_key curr_state_data;
+  let curr_state_key_size = get_state_data_key_size curr_state_data;
 
+  
+  //append req and resp
+  let append_req_resp = append_vec req resp #b_req #b_resp #p_req #p_resp;
+  
+  //get the ghost transcript
+  let curr_g_transcript = current_transcript tr0;
+  let curr_g_key = current_key tr0;
+  let curr_g_key_size = current_key_size tr0;
+  //unfold (spdm_inv c trace_ref tr0);
+  
+  //unfold (session_state_related c (current_state tr0));
 
-//Figure out the trace
-//Write that trace to trace_ref using ghost_write
-//assume the post condition of ghost_write and see if the invaraint can be proved.
+  assume_(V.pts_to curr_state_transcript (G.reveal curr_g_transcript));
+  //append req/resp to the current trascript
+  let new_transcript = append_vec curr_state_transcript append_req_resp #curr_g_transcript #(Seq.append b_req b_resp);
+  let new_g_transcript = g_append curr_g_transcript (Seq.append b_req b_resp);
+  //create a new state data record with the new transcript
+  assume_ (pure (V.length curr_state_signing_pub_key == u32_v curr_state_key_size));
 
+  let new_st = {key_size = curr_state_key_size; signing_pub_key = curr_state_signing_pub_key; session_transcript = new_transcript };
+  
+  ////creation of the ghost session data storage
+  let repr = {key_size_repr = curr_g_key_size; signing_pub_key_repr = curr_g_key; transcript = new_g_transcript};
 
-(*let init_client_perm (s:state) (b:Seq.seq u8) (key_len:u32): slprop =
-  exists* (t:trace). spdm_inv s trace_ref t ** 
-                                   pure (G_Initialized? (current_state t) /\
-                                        g_key_of_gst (current_state t) == b /\
-                                        g_key_len_of_gst (current_state t) == key_len
-                                        )
-*)
+  //Do the state change
 
-
-
-
-
-
-
+  
+  //Call parser to parse and get the measurement blocks.
+  admit()
+}
